---
title: Logic notes
categories: [ Personal, Science, Philosophy ]
---

# Elementary order theory

## Equivalence relations

**Definition 1**. *A relationship $\preceq$ over a set $A$ is an
equivalence relation if it is reflexive, symmetric, and transitive.*

**Definition 2**. *Let $\preceq$ an equivalence relationship over a set
$A$ and $x \in A$. Then the equivalence class of $x$ is denoted $[x]$
and defined as*

$$\begin{aligned}
[x] = \{y : y \in A \text{ and } y \preceq x\}
    \end{aligned}$$

This too is quite simple. For example, consider the relationship
$\preceq$ such that $a \preceq b$ means $a$ *has the same parity than*
$b$. Then $[2]$ denotes the set of all even numbers. Since the
relationship is symmetric, any $x$ such that $2 \preceq x$ satisfies
$[2] = [x]$, and this is a generalizable result (true for any
$\preceq$).

**Theorem 1**. *Let $\preceq$ an equivalence relationship over $A$ and
$x, y$ elements of $A$. Then*

$$\begin{aligned}
        &(1) ~ [x] = [y] \Leftrightarrow x \preceq y \newline 
        &(2) ~ x \not \preceq y \implies [x] \cap [y] = \emptyset
    \end{aligned}$$

***Proof.** $(1)$ is quite trivial and we skip it. To prove $(2)$,
assume $x \not \preceq y$. If $[x] \cap [y] \neq \emptyset$ then there
is some $a \in [x] \cap [y]$ such that $a \preceq x$ and $a \preceq y$.
Since $\preceq$ is transitive we have $x \preceq y$, a contradiction.
$\blacksquare$*

**Definition 3**. *The partition of any set $A$ is any family of
non-empty subsets of $A$ that are disjoint and whose union is $A$.*

**Theorem 2**. *Let $\preceq$ an equivalence relationship over a
non-empty $A$. Then the family of equivalence classes of $A$ is a
partition of $A$.*

***Proof.** We have shown any equivalence classes $[x], [y]$ such that
$[x] \neq [y]$ are disjoint. Since $x \preceq x$ for any $x \in A$ we
are guaranteed that $[x]$ is non-empty for all $A$. It follows then*

$$\begin{aligned}
\cup \ldots \cup [a_n] = A
    \end{aligned}$$

*where $[a_1], \ldots, [a_n]$ are all (distinct) equivalence classes of
$A$. $\blacksquare$*

## Order relations

**Definition 4**. *A partial order $\preceq$ over a set $P$ is a
transitive, reflexive, and anti-symmetric relation between the elements
of $P$.*

**Definition 5**. *Let $\preceq$ a relationship over $P$ and $a, b$
elements of $P$. We say $b$ covers $a$ if $a \preceq b$ and for every
$x \in P$ such that $a \preceq x$, then $b \preceq x$.*

**Example 1**. *Take the set $\{2, 4, 5, 8, 9, 12\}$. The number $4$
divides $8$ and $12$ and so does $2$. Then $4$ covers $2$ under the
relationship $\mid$ (*divides*).*

**Definition 6**. *Let $(P, \preceq)$ a partial order. A Hasse diagram
is a graph $G = (V, E)$ such that $V = P$ and
$E = \{(a, b) : a, b \in P:  a \text{ covers } b\}$.*

Simply put, a Hasse diagram is a graph containing the elements of $P$,
and whose edges denote the cover relation. In truth, Hasse diagrams are
what make clear the purpose of defining a relationship such as
\"cover\".

**Definition 7**. *Every partial order has minimal and maximal elements,
and some have maximum and minimum elements. These are defined as
follows.*

$$\begin{aligned}
        \text{max } P  = x &\iff  \langle \forall e : e \in P : e \preceq x \rangle \newline
        \text{min } P = x &\iff \langle \forall  e : e \in P : x \preceq e \rangle \newline
        \text{minimal } P = x &\iff \langle \forall  e : e \in P \land e \preceq x :
            x = e \rangle \newline
        \text{maximal } P = x &\iff \langle \forall  e : e \in P \land x \preceq e :
            x = e \rangle \newline
        \end{aligned}$$

For a visual representation of their differences, consider the following
GIF.

**Theorem 3**. *If $x$ is a maximum, then $x$ is the only maximal. If
$x$ is minimum, it is the only minimal.*

***Proof.** It trivially follows from the definitions.*

**Definition 8**. *Let $cs(x), cl(x)$ denote that $x$ is the upper or
lower bound, respectively, of a partial order $(P, \preceq )$. We say
$x$ is a supremum if and only if*

$$\begin{aligned}
        cs(x) \land \langle \forall y : cs(y) : y \geq x \rangle
    .\end{aligned}$$

*We say $x \in P$ is an infimum if and only if*

$$\begin{aligned}
        ci(x) \land \langle \forall y : ci(y) : y \leq x \rangle
    .\end{aligned}$$

A different way to understand this is to say the infimum of a partial
order is its highest lower bound, and the supremum, its smaller upper
bound.

**Definition 9**. *A lattice is a partial order where every pair of
elements has both a supremum and an infimum.*

From a graphical perspective, a lattice conforms a Hasse diagram such
that no pair of elements are unconnected.

Since any pair of elements $x, y$ in a lattice has a supremum and an
infimum, we may define two binary operators $\land, \lor,$ such that
$x \land y, x \lor
y$ denote the infimum and supremum of these elements, respectively.

In general, we use the notation $(L, \land, \lor)$ to denote a lattice
$L$. This readily conveys that we are dealing with a poset $L$ for which
$\land, \lor,$ are well-defined binary operations.

Observe that $\land, \lor$, are reflexive, commutative, and absorbent
with respect to each other. In other words,

$$\begin{aligned}
    x \lor x = x\land x = x, ~ ~ ~ x \land y = y \land x  ~ ~ ~ x \lor (x \land
    y) = x ~ ~ ~ x
    \land (x \lor y) = x\end{aligned}$$

**Definition 10**. *A lattice $(L, \lor, \land)$ is said to be bounded
if $0 \lor x = x, 1 1
    \lor x = 1$, where $0, 1$ denote the supremum and infimum of $L$.*

**Definition 11**. *We say a lattice $(L, \lor, \land)$ is complemented
if and only if for every $x \in L$ there is some $x^c \in L$ such that
$x \lor x^c = 1, x \land x^c =
    0$.*

If $(L, \lor, \land)$ is a lattice and $L$ is a poset under an order
relation $\preceq$, then the following properties are satisfied.

$$\begin{aligned}
    &x \preceq x \lor y \newline 
    &x \land y \preceq x \newline 
    &x \preceq y \iff x \lor y = y \iff x \land y = x \newline 
    &x \preceq  z \text{ and } y \preceq  w \implies (x \lor y) \preceq
    (z \lor w) \text{ and } (x \land y) \preceq (z \land w)
    &\{\text{Compatibility}\} \newline 
    &x\lor(y \land z) \preceq (x\lor y) \text{ and } x \land (y \lor z) \preceq (x \land y)
\lor (x \land z)\end{aligned}$$

**Definition 12**. *Two lattices $(L, \land, \lor), (L', \land', \lor')$
are isomorphic if there is a bijection $f : L \to L'$ such that*

$$\begin{aligned}
        f(x \lor y) = f(x) \lor' f(y) ~ ~ ~ f(x \land y) = f(x) \land' f(y)
    \end{aligned}$$

*If this is the case, we write
$(L, \land, \lor) â‰Š/ (L', \land', \lor')$.*

**Definition 13**. *A sublattice $(M, \land, \lor)$ of a lattice
$(L, \land, \lor)$ is a lattice such that $a.$ $M \subseteq L$, and $b.$
for any $x, y \in M$ we have $x
    \land y, x \lor y \in M$.*

**Definition 14**. *If a lattice is such that $x, y$ satisfy the
distributive property, then it is said to be a distributive lattice.*

**Theorem 4**. *If a lattice is distributive and bounded, then it is
necessarily complemented.*

***Proof.** TO COMPLETE.*

**Definition 15**. *A structure $(B, \lor, \land, ^c, 0, 1)$ with $B$ a
non-empty set, $^c$ a unary operator, $0, 1 \in B$, is a Boolean algebra
if and only if: $a.$ $(B,
    \lor, \land)$ is a bounded and distributive lattice, and $b.$
$x \lor x^c =
    1, x \land x^c = 0$.*

Observe that $x^c$ is not required to exist in $B$. This is why a
Boolean algebra is not readily defined as a bounded, distributive, and
complemented lattice altogether. Furthermore, in a complemented lattice,
$a^c$ is understood to be a complement of $a$ as a function of the
binary operators $\land, \lor$. In a Boolean algebra, in truth, $^c$ is
a unary operation.

**Theorem 5**. *If $(B, \lor, \land, ^c, 0, 1)$ is a Boolean algebra,
then its elements satisfy DeMorgan's laws (where $^c$ is understood to
be equivalent to negation).*

**Definition 16**. *Two Boolean algebras are isomorphic if there is a
bijection $f : B \to B'$ such that $f(0) = 0', f(1) = 1'$, and for every
$x, y \in B$ we have*

$$\begin{aligned}
        f(x \lor y) = f(x) \lor\ f(y) ~ ~ ~ f(x \land y) = f(x) \land' f(y) ~ ~
        ~ f(x^c) = f(x)^{c'}
    \end{aligned}$$

## Representation theorems

**Definition 17**. *Let $B$ a Boolean algebra. An element $a \in B$ is
an atom if $a$ covers $0$.*

We shall use $At(B)$ to denote the set of all atoms in $B$.

**Lemma 1**. *Let $B$ a finite Boolean algebra. Then any $x \in B$ is
uniquely determined as the supreme of atoms. This is, for any
$x \in B$,*

$$\begin{aligned}
        &x = \text{sup}\{a \in At(B) : a \preceq x\} \newline 
        &A \subseteq At(B) \text{ and }x = \text{sup } A \implies A = \{a \in At(B) : a
        \preceq x\}
    \end{aligned}$$

***Proof.** Let $A_x = \{ a \in At(B) : a \preceq x\}$ and $y =
    \text{sup }\{a \in At(B) : a \preceq x\} = \text{sup }A_x$.*

*(1) Since $x$ is an upper bound of $A_x$, then $y \preceq x$. If
$x \not \preceq
    y$, there is some $a \in At(B)$ such that $a \preceq x$ and
$a \not\preceq y$ (see following lemma). But this is absurd by the
definition of $y$. Then $x
    \preceq y$. Then $x = y$.*

*$(2)$ COMPLETE.*

**Lemma 2**. *Let $B$ a finite boolean algebra, and $x, y \in B$ such
that $x \not\preceq
    y$. Then there is some $a \in At(B)$ such that $a \preceq x$ and $a
    \not\preceq y$. In other words, for finite Boolean algebras, the
non-relation of two elements implies the existence of some non-common
atom.*

***Proof.** Assume $x \not \preceq y$. From this follows that $x \land
    y^c \neq 0$. Indeed, if $x \land y^c = 0$, then
$y \lor (x \land y^c) = y
    \lor 0 = y$. So
$(y \lor x) \land (y \lor y^c) = (y \lor x) \land 1 = y \lor
    x = y$, which implies $x \preceq y$, a contradiction. We then have
that $a
    \preceq x\land y^c$ for some $a \in At(B)$. It is clear that
$a \preceq x$. Assume $a \preceq y$. Then
$a \preceq x \land y^c \land y = 0$, which is absurd since $a$ is atom.
Then $x \not \preceq y$ implies there is an atom such that $a \preceq x$
and $a \not \preceq y$.*

**Theorem 6**. *Let $B$ a finite Boolean algebra. The function*

$$\begin{aligned}
        f : B &\to \mathcal{P}\big( At(B) \big) \newline 
        x &\to \{a \in At(B) : a \preceq x\}
    \end{aligned}$$

*is an isomorphism between $(B, \land, \lor, ^c, 0, 1)$ and
$(\mathcal{P}\big( At(B) \big), \cup, \cap, ^c, \emptyset, At(B))$.*

***Proof.** (1) $f$ is injective because $A_x = A_y$ implies
$\text{sup }
    A_x = \text{sup }A_y$, and by the previous lemmas we have $x = y$.
(2) $f$ is surjcetive. Indeed, let $A \subseteq At(B)$ and
$x = \text{sup }A$. We have, by the lemmas, that $A = A_x$, which
implies $f(x) = A$. $(3)$ That $f$ is an isomorphism it follows from the
following fact: TO COMPLETE.*

## Representation theorem for distributive lattices

**Definition 18**. *Let $(P, \preceq)$ a poset. We say $D \subseteq P$
is decreasing if for any $x, z \in P$ we have*

$$\begin{aligned}
        x \in D \text{ and } y \preceq z \implies z \in D
    \end{aligned}$$

We use the notation $\mathcal{D}(P)$ to denote the set of all decreasing
subsets of $P$, or
$\mathcal{D}(P) = \{ D \subseteq P : D \text{ is decreasing }\}$. It
follows that to any poset $(P, \preceq )$ there is an associated bounded
lattice $(\mathcal{D}(P), \cup, \cap, \emptyset, P)$.

**Definition 19**. *Let $L$ a bounded lattice. An element $x \in L$ is
$\lor$-irreducible if*

$$\begin{aligned}
        &x \neq 0 \newline 
        &x = y\lor z \implies x = y \text{ or } x = z, \text{ for all $y, z \in L$ }
    \end{aligned}$$

It is quite clear that any $a \in At(L)$ is $\lor$-irreducible. If $L$
is a bounded lattice, we write

$$\begin{aligned}
    Irr(L) = \{i \in L : i \text{ is irreducible }\}\end{aligned}$$

**Lemma 3**. *Let $B$ a Boolean algebra. Then $x \in B$ is
$\lor$-irreducible iff $x$ is an atom.*

Our last result will be presented without proof. A proof exists in
Tiraboschi's order theory.

**Theorem 7**. *Let $L$ a finite distributive bounded lattice. Then*

$$\begin{aligned}
        f : L &\to \mathcal{D} \big( Irr(L) \big) \newline 
        x &\to \{y \in Irr(L) : y \preceq x\}
    \end{aligned}$$

*is an isomorphism between $(L, \lor, \land, 0, 1)$ and
$(\mathcal{D}\big(
    Irr(L) \big), \cup, \cap, \emptyset, Irr(L))$.*

# Problems

**Problem 1**. *Let $P$ a poset. Prove that if $P$ has a maximum element
$x$, then it $x$ is the only maximal.*

Assume $x$ is the maximum of $P$. That $x$ is maximal is easy to observe
due to the anti-symmetric nature of $\preceq$. Indeed, since
$a \preceq x$ for all $x \in
a$, it follows $x \not \preceq a$ for all $a \neq x$. (This is an
alternative way of interpreting maximality. Indeed,
$x \preceq a \implies x = x$ is equivalent to the aforementioned
property.) That it is the only maximal is not hard to observe. Simply
assume some other maximal $x'$ exists. By definition, $x' \preceq x$.
Then $x'$ is not maximal, a contradiction. $\blacksquare$

**Problem 2**. *If $P$ is finite and has a unique maximal $x$, then $x$
is the maximum.*

Assume a unique maximal $m$. Assume there is some $x \in P$ such that
$x \not
\preceq m$. Let $X = \{y \in P : x \preceq y\}$. Since $P$ is finite so
is $X$, and then there is a maximal element in $X$, call it $m'$.
Observe that $m'$ is also a maximal of $P$ (by definition). That
$m' \neq m$ follows from the assumption $x \preceq m$. Then $m$ is a
unique maximal, which contradicts our assumption. Then if $m$ is a
unique maximal, every $x$ in $P$ must satisfy $x \preceq m$, or
equivalently $m$ is also the maximum. $\blacksquare$

**Problem 3**. *Let $f: P \to Q$ be an isomorphism between posets
$P, Q$. Show that if $Q$ has some minimal, then so does $P$.*

By definition, $f$ is a bijection and therefore it has an inverse
$f^{-1}$. Let $m$ denote the minimal of $Q$. Then $f^{-1}(m) = m'$ must
be a minimal element of $P$. Simply observe that, for all $x$ in $Q$,

$$\begin{aligned}
    m \preceq x  \implies f(m) \preceq f(x) ~  ~  ~\blacksquare\end{aligned}$$

**Problem 4**. *Let $P$ a poset such that $\text{sup } \{a, b\}$ exists
for all $a, b \in
    P$. Show that $\text{sup } S$ exists for all $S \subseteq P$ that
is finite and non-empty.*

First of all, observe that any $S \subseteq P$ with $|S| = 1$ has a
supremum as an immediate consequence of the definition---it is the very
element of $S$. Now let
$f(\{a_1, \ldots, a_k\}) = \text{sup } \{f(\{a_1, \ldots, a_{k - 1}\}), a_k\}$
a recursive function for the supremum of a set. We shall prove this
function to be well-defined for any $\{a_1, \ldots, a_k\} \subseteq S$.

*(1)* Let $S \subseteq P$ such that $|S| = 2$. Then
$f(S) = \text{sup }\{s_1,
s_2\}$ which exists by assumption.

*(2)* Let $S \subseteq P$ be such that $|S| = k + 1$, with $k \in
\mathbb{N}, k + 1 > 2$. Then
$f(S) = \text{sup } \{f(\{s_1, \ldots, s_k\}), a_{k + 1}\} = \text{sup }
\{x, a_{k +1}\}$. Here, $x = f(\{s_1, \ldots, s_k\})$ exists by
inductive hypothesis and $\text{sup } \{x, a_{k + 1}\}$ exists by
assumption.

*(3)* By induction, every finite, non-empty $S \subseteq P$ has a
supremum. $\blacksquare$

**Problem 5**. *Let $P$ be a total order. Is it valid to say $P$ has at
least one maximal element?*

Since $P$ a total order, for every $a, b \in P$ we have $a \preceq b$ or
$b
\preceq a$. If $P$ is infinite, it is quite clear the statement holds
not. If $P$ is finite, the statement must be true, and it can be proven
inductively.

*(1)* Let $\{a, b\}$ a total order. Then either $a \preceq b$ or
$b \preceq
a$. In the first case, $b$ is maximal; in the second, $a$ is maximal.
Then any total order $(T, \preceq)$ with $|T| = 2$ has a maximal
element.

*(2)* Let $(T, \preceq)$ a total order with $|T| = k + 1, k + 1 > 2$. By
inductive hypothesis, $T - \{t_{k + 1}\}$ has at least a maximal element
$m$. Since $T$ is a total order, then $m \preceq t_{k + 1}$ or
$t _{ k + 1 } \preceq m$. In the second case, it immediately follows
that $m$ is a maximal element of $T$. If $m \preceq t_{k+1}$, the
assumption $t_{k + 1} \preceq x$ for some $x \in
T - \{t_{k + 1}\}$ implies $m \preceq x$, which is a contradiction. Then
$t_{k +
1}$ precedes only itself. Then $t_{k + 1}$ is maximal.

*(3)* Any finite total order has a maximal element. $\blacksquare$

**Problem 6**. *Let $B$ a Boolean algebra under the order $\preceq$.
Show that $(x^c)^c = x$.*

By definition, for every $x \in B$ there is a unique complement $x^c$
such that $x \lor x^c = 1, x \land x^c = 0$. Remember that the
$\lor, \land$ operators are commutative. Then $x \lor
x^c = x^c \lor x = 1, x \land x^c = x^c \land x = 0$. Then $x$ is a
complement of $x^c$. Then $(x^c)^c = x$. $\blacksquare$

**Problem 7**. *Now show $x \preceq y \iff y^c \preceq x^c$.*

Assume $x \preceq y$. Then

$$\begin{aligned}
    y^c &\preceq y^c \land (y^c \lor x^c) &\{\text{Reflex.,
    absorption}\}\newline 
        y^c &\preceq y^c \land (y \land x)^c & \{\text{De Morgan}\}\newline 
        y^c &\preceq y^c \land x^c & \{\text{Assumption}\} \newline 
        y^c &\preceq y^c \land x^c \preceq x^c &\{ a \land b
    \preceq a\} \newline 
            y^c &\preceq x^c  ~ \blacksquare &\{\text{Transitivity}\}
.\end{aligned}$$

Now assume $x^c \preceq y^c$. We shall proceed in a similar manner, now
remembering that we have shown $(a^c)^c = a$. In particular, observe
that by De Morgan's law we have

$$\begin{aligned}
    a \lor b = (a^c)^c \lor (b^c)^c = (a^c \land b^c)^c
.\end{aligned}$$

Now,

$$\begin{aligned}
    x &\preceq x \land (x \lor y) &\{\text{Absorption}\} \newline 
    x &\preceq x \land (x^c \land y^c)^c &\{\text{Eq. (1)}\} \newline 
    x &\preceq x \land (y^c)^c &\{\text{Assumption}\} \newline 
    x &\preceq x \land y \preceq y \newline 
    x &\preceq y ~ \blacksquare
.\end{aligned}$$

**Problem 8**. *Show $y \land z = 0 \iff y \preceq z^c$.*

Assume $y \land z = 0$. This problem can be solved by dividing it in two
cases. Either $y \lor z = 1$ or $y \lor z \neq 1$.

*(1) $\big( y \lor z = 1 \big)$ :* If $y \lor z = 1$ then $y = z^c$
(since $y \land z = 0$ by assumption). Then by reflexivity $y
\preceq z^c$.

*(2) $\big( y \lor z \neq 1 \big)$ :* Observe that since $y
\lor z \neq 1$ we have $y \neq 1$. Now it follows

$$\begin{aligned}
    y \land (z \lor z^c) &= y &\{z \lor z^c = 1\}\newline 
    (y \land z) \lor (y \land z^c) &= y &\{\text{Distr.}\} \newline 
    0 \lor (y \land z^c) &= y &\{\text{Assumption}\} \newline 
    y \land z^c &= y &\{0 \lor a = a\} \newline 
    y &\preceq z^c &\{a \land b = a \Rightarrow a \preceq b\}
.\end{aligned}$$

**Problem 9**. *If $x \preceq y$ and $y \land z = 0$, then
$z \preceq x^c$.*

Given our previous result, it would suffice to show that from the
premises follows $x \land z = 0$. Now, assume $x \land z \neq 0$. Since
$x \preceq y$, we have $x \land y = x$ and then $(x \land y)
\land z \neq 0 \Rightarrow x \land (y \land z) \neq 0$. But $y
\land z = 0$ and then we arrive at $x \land 0 \neq 0$, which is a
contradiction. Then $x \land z = 0$, which implies $z \preceq x^c$.
